Graph_Theory/Dgraph.thy
@@ -1,5 +1,7 @@
 theory Dgraph
-  imports AGF.DDFS
+  imports
+    AGF.DDFS
+    "HOL-Data_Structures.Set_Specs"
 begin
 
 section \<open>Graphs\<close>
@@ -31,12 +33,12 @@ proof -
     by blast
 qed
 
-section \<open>Neighborhood\<close>
+subsection \<open>Neighborhood\<close>
 
 definition out_neighborhood :: "'a dgraph \<Rightarrow> 'a \<Rightarrow> 'a set" where
   "out_neighborhood G u \<equiv> {v \<in> dVs G. (u, v) \<in> G}"
 
-lemma (in dgraph) in_out_neighborhood_iff_edge:
+lemma (in dgraph) mem_out_neighborhood_iff_edge:
   shows "v \<in> out_neighborhood G u \<longleftrightarrow> (u, v) \<in> G"
   using dVsI(2)
   by (auto simp add: out_neighborhood_def)
@@ -49,5 +51,47 @@ lemma (in finite_dgraph) out_neighborhood_finite:
   shows "finite (out_neighborhood G u)"
   using out_neighborhood_subset_vertices vertices_finite
   by (rule finite_subset)
+
+section \<open>\<close>
+
+locale finite_dgraph_tbd =
+  finite_dgraph G +
+  Set_by_Ordered where insert = insert
+  for
+    G :: "'a::linorder dgraph" and
+    insert :: "'a \<Rightarrow> 's \<Rightarrow> 's" +
+  fixes out_neighborhood :: "'a \<Rightarrow> 's"
+  assumes invar_out_neighborhood: "v \<in> dVs G \<Longrightarrow> invar (out_neighborhood v)"
+  assumes isin_out_neighborhood_iff_edge: "invar (out_neighborhood u) \<Longrightarrow> isin (out_neighborhood u) v \<longleftrightarrow> (u, v) \<in> G"
+
+lemma (in finite_dgraph_tbd) mem_out_neighborhood_iff_edge:
+  assumes "invar (out_neighborhood u)"
+  shows "v \<in> set (out_neighborhood u) \<longleftrightarrow> (u, v) \<in> G"
+  using assms isin_out_neighborhood_iff_edge
+  by (simp add: invar_def isin set_def)
+
+lemma (in finite_dgraph_tbd) mem_out_neighborhood_if_edge:
+  assumes "(u, v) \<in> G"
+  shows "v \<in> set (out_neighborhood u)"
+proof -
+  have "u \<in> dVs G"
+    using assms
+    by (intro dVsI(1))
+  hence "invar (out_neighborhood u)"
+    by (intro invar_out_neighborhood)
+  thus ?thesis
+    using assms
+    by (simp add: mem_out_neighborhood_iff_edge)
+qed
+
+lemma (in finite_dgraph_tbd) out_neighborhood_subset_vertices:
+  assumes "invar (out_neighborhood u)"
+  shows "set (out_neighborhood u) \<subseteq> dVs G"
+  using assms
+  by (auto simp add: mem_out_neighborhood_iff_edge intro: dVsI(2))
+
+lemma (in finite_dgraph_tbd) out_neighborhood_finite:
+  shows "finite (set (out_neighborhood u))"
+  by (simp add: set_def)
 
 end
