Misc.thy
@@ -1,8 +1,0 @@
-theory Misc
-  imports
-    Queue_Specs
-begin
-
-section \<open>Queues\<close>
-
-end
